proof/agp32_MEM_CorrectScript.sml
@@ -889,10 +889,8 @@ QED
 (** command **)
 (** StoreMem **)
 Theorem agp32_Rel_ag32_command_correct_write_mem_WB_enable:
-  !fext fbits a t I.
-    is_mem fext_accessor_circuit (agp32 fext fbits) fext ==>
-    is_sch I (agp32 fext fbits) a ==>
-    I (5, SUC t) <> NONE ==>
+  !fext fbits a t.
+    is_mem fext_accessor_circuit (agp32 fext fbits) fext ==>   
     enable_stg 5 (agp32 fext fbits t) ==>
     (agp32 fext fbits (SUC t)).WB.WB_opc = 2w ==>
     (agp32 fext fbits (SUC t)).command = 3w
@@ -903,7 +901,6 @@ Proof
   `(fext t).error = 0w` by fs [is_mem_def,mem_no_errors_def] >>
   `s.MEM.MEM_opc = 2w` by METIS_TAC [agp32_WB_opc_MEM_opc_when_WB_enabled,Abbr `s`] >>
   `s.MEM.MEM_write_mem` by METIS_TAC [Abbr `s`,agp32_MEM_write_mem_MEM_opc_2w] >>
-  `I' (5,SUC t) = I' (4,t)` by fs [is_sch_def,is_sch_writeback_def] >>
   `s.state = 0w`
     by (fs [Abbr `s`,enable_stg_def] >> Cases_on_word_value `(agp32 fext fbits t).state` >>
         METIS_TAC [agp32_WB_state_flag_and_state,agp32_state_impossible_values]) >>
@@ -914,10 +911,8 @@ QED
 
 (** StoreMemByte **)
 Theorem agp32_Rel_ag32_command_correct_write_mem_byte_WB_enable:
-  !fext fbits a t I.
+  !fext fbits a t.
     is_mem fext_accessor_circuit (agp32 fext fbits) fext ==>
-    is_sch I (agp32 fext fbits) a ==>
-    I (5, SUC t) <> NONE ==>
     enable_stg 5 (agp32 fext fbits t) ==>
     (agp32 fext fbits (SUC t)).WB.WB_opc = 3w ==>
     (agp32 fext fbits (SUC t)).command = 3w
@@ -928,7 +923,6 @@ Proof
   `(fext t).error = 0w` by fs [is_mem_def,mem_no_errors_def] >>
   `s.MEM.MEM_opc = 3w` by METIS_TAC [agp32_WB_opc_MEM_opc_when_WB_enabled,Abbr `s`] >>
   `s.MEM.MEM_write_mem_byte` by METIS_TAC [Abbr `s`,agp32_MEM_write_mem_byte_MEM_opc_3w] >>
-  `I' (5,SUC t) = I' (4,t)` by fs [is_sch_def,is_sch_writeback_def] >>
   `s.state = 0w`
     by (fs [Abbr `s`,enable_stg_def] >> Cases_on_word_value `(agp32 fext fbits t).state` >>
         METIS_TAC [agp32_WB_state_flag_and_state,agp32_state_impossible_values]) >>
@@ -940,10 +934,8 @@ QED
 
 (** LoadMem **)
 Theorem agp32_Rel_ag32_command_correct_read_mem_WB_enable:
-  !fext fbits a t I.
+  !fext fbits a t.
     is_mem fext_accessor_circuit (agp32 fext fbits) fext ==>
-    is_sch I (agp32 fext fbits) a ==>
-    I (5, SUC t) <> NONE ==>
     enable_stg 5 (agp32 fext fbits t) ==>
     (agp32 fext fbits (SUC t)).WB.WB_opc = 4w ==>
     (agp32 fext fbits (SUC t)).command = 2w
@@ -954,7 +946,6 @@ Proof
   `(fext t).error = 0w` by fs [is_mem_def,mem_no_errors_def] >>
   `s.MEM.MEM_opc = 4w` by METIS_TAC [agp32_WB_opc_MEM_opc_when_WB_enabled,Abbr `s`] >>
   `s.MEM.MEM_read_mem` by METIS_TAC [Abbr `s`,agp32_MEM_read_mem_MEM_opc_4w_5w] >>
-  `I' (5,SUC t) = I' (4,t)` by fs [is_sch_def,is_sch_writeback_def] >>
   `s.state = 0w`
     by (fs [Abbr `s`,enable_stg_def] >> Cases_on_word_value `(agp32 fext fbits t).state` >>
         METIS_TAC [agp32_WB_state_flag_and_state,agp32_state_impossible_values]) >>
@@ -965,10 +956,8 @@ QED
 
 (** LoadMemByte **)
 Theorem agp32_Rel_ag32_command_correct_read_mem_byte_WB_enable:
-  !fext fbits a t I.
+  !fext fbits a t.
     is_mem fext_accessor_circuit (agp32 fext fbits) fext ==>
-    is_sch I (agp32 fext fbits) a ==>
-    I (5, SUC t) <> NONE ==>
     enable_stg 5 (agp32 fext fbits t) ==>
     (agp32 fext fbits (SUC t)).WB.WB_opc = 5w ==>
     (agp32 fext fbits (SUC t)).command = 2w
@@ -979,13 +968,39 @@ Proof
   `(fext t).error = 0w` by fs [is_mem_def,mem_no_errors_def] >>
   `s.MEM.MEM_opc = 5w` by METIS_TAC [agp32_WB_opc_MEM_opc_when_WB_enabled,Abbr `s`] >>
   `s.MEM.MEM_read_mem` by METIS_TAC [Abbr `s`,agp32_MEM_read_mem_MEM_opc_4w_5w] >>
-  `I' (5,SUC t) = I' (4,t)` by fs [is_sch_def,is_sch_writeback_def] >>
   `s.state = 0w`
     by (fs [Abbr `s`,enable_stg_def] >> Cases_on_word_value `(agp32 fext fbits t).state` >>
         METIS_TAC [agp32_WB_state_flag_and_state,agp32_state_impossible_values]) >>
   `(fext t).ready`
     by (fs [Abbr `s`,enable_stg_def] >> METIS_TAC [agp32_WB_state_flag_and_fext_ready]) >>
   fs [agp32_next_state_def,Abbr `s`,agp32_MEM_read_mem_others_F]
+QED
+
+(** command when the WB is disabled and fext is ready at the previous cycle **)
+Theorem agp32_Rel_ag32_command_correct_WB_disable_fext_ready:
+  !fext fbits a t I.
+    is_mem fext_accessor_circuit (agp32 fext fbits) fext ==>
+    ~enable_stg 5 (agp32 fext fbits t) ==>
+    (fext t).ready ==>
+    (agp32 fext fbits (SUC t)).WB.WB_opc <> 16w ==>
+    (agp32 fext fbits (SUC t)).command = 0w
+Proof
+  rw [] >> Q.ABBREV_TAC `s = agp32 fext fbits t` >>
+  `(agp32 fext fbits (SUC t)).command = (agp32_next_state (fext t) s s).command`
+    by fs [agp32_command_state_updated_by_agp32_next_state] >>
+  `(fext t).error = 0w` by fs [is_mem_def,mem_no_errors_def] >>
+  Cases_on_word_value `s.state` >-
+   fs [Abbr `s`,agp32_state_impossible_values] >-
+   fs [Abbr `s`,agp32_state_impossible_values] >-
+   METIS_TAC [Abbr `s`,agp32_state_impossible_5_no_fext_error] >-
+   (`s.command = 0w` by fs [agp32_state_4_command_0,Abbr `s`] >>
+    fs [agp32_next_state_def] >>
+    IF_CASES_TAC >> fs []) >-
+   METIS_TAC [agp32_state_3_WB_opc_16,Abbr `s`] >-
+   fs [agp32_next_state_def] >-
+   fs [agp32_next_state_def] >>
+  fs [enable_stg_def,Abbr `s`] >>
+  METIS_TAC [agp32_ready_not_WB_state_flag_state_not_0]
 QED
 
 
